%% LyX 2.1.4 created this file.  For more info, see http://www.lyx.org/.
%% Do not edit unless you really know what you are doing.
\documentclass[english]{article}
\usepackage[T1]{fontenc}
\usepackage[latin9]{inputenc}
\usepackage{geometry}
\geometry{verbose,tmargin=2cm,bmargin=2cm,lmargin=2cm,rmargin=2cm}
\usepackage{amsmath}
\usepackage{babel}
\begin{document}

\title{Simple resistive drift instability}

\maketitle

\section{Equations}

Normalized equations:
\begin{align*}
\frac{\partial n}{\partial t} & =-\frac{\partial\phi}{\partial z}\frac{\partial n_{0}}{\partial x}=\frac{1}{L_{n}}\frac{\partial\phi}{\partial z}\\
\frac{\partial w}{\partial t} & =\frac{\partial j}{\partial y}\\
\nabla_{\perp}^{2}\phi & =w\\
j & =\frac{1}{\mu\eta}\left(\frac{\partial n}{\partial y}-\frac{\partial\phi}{\partial y}\right)
\end{align*}



\section{Dispersion relation}

In Fourier space, with $\omega_{*}=\frac{k_{z}}{L_{n}}$:
\begin{align*}
(-i\omega)n & =\frac{1}{L_{n}}(ik_{z})\phi=i\omega_{*}\phi\\
(-i\omega)w & =(ik_{\|})j\\
-k_{\perp}^{2}\phi & =w\\
j & =\frac{(ik_{\|})}{\mu\eta}(n-\phi)
\end{align*}
\begin{align*}
\omega n & =-\omega_{*}\phi\\
\omega k_{\perp}^{2}\phi & =k_{\|}j\\
j & =\frac{ik_{\|}}{\mu\eta}(n-\phi)
\end{align*}
\begin{align*}
\omega k_{\perp}^{2}\phi & =\frac{ik_{\|}^{2}}{\mu\eta}(n-\phi)\\
\left(\omega k_{\perp}^{2}+i\frac{k_{\|}^{2}}{\mu\eta}\right)\phi & =\frac{ik_{\|}^{2}}{\mu\eta}n\\
\omega\left(\omega k_{\perp}^{2}+i\frac{k_{\|}^{2}}{\mu\eta}\right) & =-\frac{i\omega_{*}k_{\|}^{2}}{\mu\eta}\\
\omega^{2}k_{\perp}^{2}+i\frac{k_{\|}^{2}}{\mu\eta}\omega+\frac{i\omega_{*}k_{\|}^{2}}{\mu\eta} & =0\\
\mu\eta\omega^{2}k_{\perp}^{2}+ik_{\|}^{2}\omega+i\omega_{*}k_{\|}^{2} & =0
\end{align*}
\begin{align}
\omega & =\frac{-ik_{\|}^{2}\pm\sqrt{-k_{\|}^{4}-4i\mu\eta\omega_{*}k_{\|}^{2}k_{\perp}^{2}}}{2\mu\eta k_{\perp}^{2}}\nonumber \\
\omega & =\frac{-ik_{\|}^{2}\pm i\sqrt{k_{\|}^{4}+4i\mu\eta\omega_{*}k_{\|}^{2}k_{\perp}^{2}}}{2\mu\eta k_{\perp}^{2}}\label{eq:omega}
\end{align}
Taking positive root for growing solution, and noting $\sqrt{A}\pm\sqrt{B}=\sqrt{(\sqrt{A}\pm\sqrt{B})^{2}}=\sqrt{A+B\pm2\sqrt{AB}}$
(this method loses the sign of $\sqrt{A}\pm\sqrt{B}$, so note that
$\Re(\omega)>0$ by Taylor expanding (\ref{eq:omega})). 
\begin{align*}
\Re(\omega) & =\frac{1}{2}(\omega+\omega^{\dagger})\\
 & =\frac{-ik_{\|}^{2}+i\sqrt{k_{\|}^{4}+4i\mu\eta\omega_{*}k_{\|}^{2}k_{\perp}^{2}}+ik_{\|}^{2}-i\sqrt{k_{\|}^{4}-4i\mu\eta\omega_{*}k_{\|}^{2}k_{\perp}^{2}}}{4\mu\eta k_{\perp}^{2}}\\
 & =\frac{i\sqrt{k_{\|}^{4}+4i\mu\eta\omega_{*}k_{\|}^{2}k_{\perp}^{2}}-i\sqrt{k_{\|}^{4}-4i\mu\eta\omega_{*}k_{\|}^{2}k_{\perp}^{2}}}{4\mu\eta k_{\perp}^{2}}\\
 & =-\frac{i\sqrt{k_{\|}^{4}+4i\mu\eta\omega_{*}k_{\|}^{2}k_{\perp}^{2}+k_{\|}^{4}-4i\mu\eta\omega_{*}k_{\|}^{2}k_{\perp}^{2}-2\sqrt{(k_{\|}^{4}+4i\mu\eta\omega_{*}k_{\|}^{2}k_{\perp}^{2})(k_{\|}^{4}-4i\mu\eta\omega_{*}k_{\|}^{2}k_{\perp}^{2})}}}{4\mu\eta k_{\perp}^{2}}\\
 & =-\frac{i\sqrt{2k_{\|}^{4}-2\sqrt{(k_{\|}^{8}+16(\mu\eta\omega_{*}k_{\|}^{2}k_{\perp}^{2})^{2}}}}{4\mu\eta k_{\perp}^{2}}\\
 & =-\frac{\sqrt{2\sqrt{(k_{\|}^{8}+16(\mu\eta\omega_{*}k_{\|}^{2}k_{\perp}^{2})^{2}}-2k_{\|}^{4}}}{4\mu\eta k_{\perp}^{2}}
\end{align*}
\begin{align*}
\Im(\omega) & =\frac{1}{2i}(\omega-\omega^{\dagger})\\
 & =\frac{-ik_{\|}^{2}+i\sqrt{k_{\|}^{4}+4i\mu\eta\omega_{*}k_{\|}^{2}k_{\perp}^{2}}-ik_{\|}^{2}+i\sqrt{k_{\|}^{4}-4i\mu\eta\omega_{*}k_{\|}^{2}k_{\perp}^{2}}}{4i\mu\eta k_{\perp}^{2}}\\
 & =\frac{-2k_{\|}^{2}+\sqrt{k_{\|}^{4}+4i\mu\eta\omega_{*}k_{\|}^{2}k_{\perp}^{2}}+\sqrt{k_{\|}^{4}-4i\mu\eta\omega_{*}k_{\|}^{2}k_{\perp}^{2}}}{4\mu\eta k_{\perp}^{2}}\\
 & =\frac{-2k_{\|}^{2}+\sqrt{k_{\|}^{4}+4i\mu\eta\omega_{*}k_{\|}^{2}k_{\perp}^{2}+k_{\|}^{4}-4i\mu\eta\omega_{*}k_{\|}^{2}k_{\perp}^{2}+2\sqrt{(k_{\|}^{4}+4i\mu\eta\omega_{*}k_{\|}^{2}k_{\perp}^{2})(k_{\|}^{4}-4i\mu\eta\omega_{*}k_{\|}^{2}k_{\perp}^{2})}}}{4\mu\eta k_{\perp}^{2}}\\
 & =\frac{-2k_{\|}^{2}+\sqrt{2k_{\|}^{4}+2\sqrt{(k_{\|}^{8}+16(\mu\eta\omega_{*}k_{\|}^{2}k_{\perp}^{2})^{2}}}}{4\mu\eta k_{\perp}^{2}}
\end{align*}



\section{Mode structure}

If $n$ is initially
\[
n=a\cos(k_{\|}y+k_{\perp}z)
\]
then as
\begin{align*}
w & =-k_{\perp}^{2}\phi\\
 & =k_{\perp}^{2}\frac{\omega}{\omega_{*}}n
\end{align*}
$w$ is initially
\[
w=a\frac{k_{\perp}^{2}}{\omega_{*}}\left(\Re(\omega)\cos(k_{\|}y+k_{\perp}z)-\Im(\omega)\sin(k_{\|}y+k_{\perp}z)\right)
\]

\end{document}
